experimenting with frames

Intermediate/Global.lean
@@ -8,27 +8,74 @@ open Lilac
 
 namespace Intermediate
 
+structure DataDeclFrame where
+  name : String
+  kind : Core.Kind
+  ctors : (n : Nat) × Vec (String × Core.SpineTy) n
+
+structure DefnFrame where
+  name : String
+  type : Core.Ty
+  term : Surface.Term
+
+structure ClassDeclFrame where
+  name : String
+  kind : Core.Kind
+  fds : List (String × Core.SpineTy)
+  scs : List (String × Core.SpineTy)
+  mths : List (String × Core.SpineTy)
+
+
+structure InstDeclFrame where
+  iname : String -- odata name
+  cls_name : String
+  kcU : Nat
+  kcE : Nat
+  Tc : Nat
+  kindsU : Vec Core.Kind kcU
+  kindsE : Vec Core.Kind kcE
+  inst_ty : Vec Core.Ty Tc
+  fds : List (String × (m : Nat) × Core.Pattern m × Surface.Term)
+  scs : List (String × (m : Nat) × Core.Pattern m × Surface.Term)
+  mths : List (String × (m : Nat) × Core.Pattern m × Surface.Term)
+
 /-- Staged Global that contains Surface level terms, but compiled types and kinds -/
 inductive Global : Type where
-| data : (n : Nat) -> String -> Core.Kind -> Vec (String × Core.SpineTy) n -> Global
-| defn : String -> Core.Ty -> Surface.Term -> Global
+| data : DataDeclFrame -> Global
+| defn : DefnFrame -> Global
 -- | classDecl : {mc kc fc : Nat} -> String -> Vec Kind kc -> Vec (String × Fin kc × Fin kc) fc ->  Vec (String × Ty) mc -> Global
-| odata : String -> Core.Kind -> Global
-| openm : String -> String -> Core.SpineTy -> Global
+| classDecl : ClassDeclFrame -> Global
+-- | odata : String -> Core.Kind -> Global
+-- | openm : String -> Core.SpineTy -> Global
 -- | instDecl : {kc mc : Nat} -> String -> String -> Vec Ty kc -> Vec (String × Term) mc -> Global
-| octor  : String -> Core.SpineTy -> Global
-| inst : {m : Nat} -> String -> String -> Core.Pattern m -> Surface.Term -> Global
+-- | octor  : String -> Core.SpineTy -> Global
+-- | inst : {m : Nat} -> String -> Core.Pattern m -> Surface.Term -> Global
+| instDecl : InstDeclFrame -> Global
+
 
 
 def Global.repr (_ : Nat) : (a : Global) -> Std.Format
-| .data _ s K ctors =>
+| .data ⟨s, K, ⟨_, ctors⟩⟩ =>
   ".data " ++ s ++ " : " ++ Core.Kind.repr max_prec K  ++ " where " ++ Std.Format.line
      ++ Std.Format.nest 4 (ctors.reprPrec 0)
-| .odata n K => ".odata " ++ n ++ " " ++ K.repr max_prec
-| .openm n cls ty => ".openm " ++ n ++ "⟨" ++ cls ++ "⟩"++ " : " ++ Core.SpineTy.repr ty
-| .defn n T t => ".defn " ++ n ++ " " ++ T.repr max_prec ++ Std.Format.line ++ t.repr max_prec
-| .inst n cls p t => ".inst " ++ n ++ " " ++ cls ++ " " ++ p.repr ++ " => " ++ t.repr max_prec
-| .octor n ty => ".octor " ++ n ++ " " ++ Core.SpineTy.repr ty
+| .defn ⟨n, T, t⟩ => ".defn " ++ n ++ " " ++ T.repr max_prec ++ Std.Format.line ++ t.repr max_prec
+| .classDecl ⟨s, K, fds, scs, mths⟩ => "classDecl " ++
+  s ++ " " ++ K.repr max_prec ++ Std.Format.line
+  ++ fds.repr max_prec ++ Std.Format.line
+  ++ scs.repr max_prec ++ Std.Format.line
+  ++ mths.repr max_prec ++ Std.Format.line
+
+-- | .odata n K => ".odata " ++ n ++ " " ++ K.repr max_prec
+-- | .openm n ty => ".openm " ++ n ++ " : " ++ Core.SpineTy.repr ty
+
+| .instDecl ⟨s, cls_name, _, _, _, Ks1, Ks2, tys, fds, scs, mths⟩ => "instDecl " ++
+  s ++ " " ++ cls_name ++ " " ++ tys.repr max_prec ++ Std.Format.line
+  ++ fds.repr max_prec ++ Std.Format.line
+  ++ scs.repr max_prec ++ Std.Format.line
+  ++ mths.repr max_prec ++ Std.Format.line
+
+-- | .inst n p t => ".inst " ++ n ++ " " ++ p.repr ++ " => " ++ t.repr max_prec
+-- | .octor n ty => ".octor " ++ n ++ " " ++ Core.SpineTy.repr ty
 
 @[simp]
 instance instRepr_Global : Repr Global where
@@ -60,23 +107,34 @@ def Entry.kind : Entry -> Option Core.Kind
 | odata _ K => K
 | _ => none
 
+
+
 def lookup (x : String) : GlobalEnv -> Option Entry
 | [] => none
-| .cons (.data _ y K ctors) tl =>
+| .cons (.data ⟨y, K, ⟨_, ctors⟩⟩) tl =>
   let ctors' := Vec.map
     (λ ((z, A), i) => if x == z then some (Entry.ctor z i A) else none)
     (Vec.zipIdx ctors)
   if x == y then return .data y K ctors
   else Vec.foldl Option.or (lookup x tl) ctors'
-| .cons (.odata y a) tl =>
-  if x == y then return .odata y a else lookup x tl
-| .cons (.openm y cls a) tl =>
-  if x == y then return .openm y cls a else lookup x tl
-| .cons (.defn y a b) tl =>
+| .cons (.defn ⟨y, a, b⟩) tl =>
   if x == y then return .defn y a b else lookup x tl
-| .cons (.inst _ _ _ _) tl => lookup x tl
-| .cons (.octor y a) tl =>
-  if x == y then return .octor y a else lookup x tl
+| .cons (.classDecl ⟨cls_name, K, fds, scs, mths⟩) tl =>
+  if x == cls_name then return (.odata cls_name K)
+  else match h : mths.findIdx? (λ ⟨n, _⟩ => x == n) with
+       | none => lookup x tl
+       | some i => match mths[i]? with
+                   | some ⟨x, spTy⟩ => return .openm x cls_name spTy
+                   | none => lookup x tl
+-- | .cons (.odata y a) tl =>
+--   if x == y then return .odata y a else lookup x tl
+-- | .cons (.openm y a) tl =>
+--   if x == y then return .openm y a else lookup x tl
+| .cons (.instDecl ⟨iname, cls_name, k1, k2, k3, Ks1, Ks2, tys, fds, scs, mths⟩) tl =>
+  if x == iname then return (.octor iname ⟨k1, Ks1, k2, Ks2, k3, tys, (gt#cls_name).mkApps_nats (List.range k1).reverse⟩)
+  else lookup x tl
+-- | .cons (.octor y a) tl =>
+--   if x == y then return .octor y a else lookup x tl
 
 def Entry.ctor? (data : String) : DataConst -> Entry -> Bool
 | .cls, ctor _ _ ⟨_, _, _, _, _, _, T⟩ | .opn, octor _ ⟨_, _, _, _, _, _, T⟩ =>
